ProofMining/Util.lean
@@ -5,6 +5,11 @@ class Mem (α : outParam $ Type u) (γ : Type v) where
 
 infix:50 " ∈ " => Mem.mem
 
+/-
+  Missing stuff about lists.
+  Much of this is translated ad litteram from Lean3 mathlib
+-/
+
 namespace List
 
   def mem (a : α) : List α → Prop
@@ -20,3 +25,9 @@ namespace List
   | a :: _, 0 => a
   | _ :: l, n + 1 => nth l n
 
+  inductive Sublist : List α → List α → Prop 
+  | slnil : Sublist [] []
+  | cons : Sublist x y → Sublist x (a :: y)
+  | cons₂ : Sublist x y → Sublist (a :: x) (a :: y)
+
+  infix:50 " <+ " => Sublist
